Rustv/Tests/ex/Cell.thy
@@ -1,0 +1,110 @@
+theory Cell
+  imports Simpl.Vcg "Rust-Verification.Rustv"
+begin
+
+text \<open>Formalization of Cell<T>. In this theory, we interpret &Cell<T> as
+a SharedReadWrite pointer to the location.\<close>
+
+(* In this theory, we are translating Rust assignments of the form of
+ * *dst = *src;
+ * as follows (Note that we are ignoring Drop semantics):
+ *)
+abbreviation copy_betw_places where
+  "copy_betw_places src dst ==
+     Guard invalid_ref {s. writable (dst s) s \<and> readable (src s) s}
+      (Basic (\<lambda>s. pop_tags (dst s) s);;
+      Basic (\<lambda>s. pop_tags (src s) s);;
+      Basic (\<lambda>s. (let v = memread (src s) s in memwrite (dst s) v s)))"
+
+record cell_env = globals_ram +
+  self :: tagged_ref
+  return :: tagged_ref
+
+record cell_set_env = cell_env +
+  val :: tagged_ref
+
+record cell_swap_env = cell_env +
+  other :: tagged_ref
+  tmp :: tagged_ref \<comment> \<open>inlining local variable for ptr::swap\<close>
+
+(* TODO: Current definition demands only read grant of argument, but it should be owner grant
+ * because Cell::set moves the argument.
+ *)
+definition cell_set_body :: "(cell_set_env, 'p, rust_error) com" where
+  "cell_set_body == copy_betw_places val self"
+
+(* TODO: We need to define a "calling convention" for handling arguments/return value.
+ *)
+definition cell_get_body :: "(cell_env, 'p, rust_error) com" where
+  "cell_get_body == copy_betw_places self return"
+
+text \<open>The implementation of Cell::swap is basically along the following lines
+(inlining ptr::swap):
+
+``` rust
+if ptr::eq(self, other) {
+  return
+}
+
+let tmp = uninit();
+*tmp = *self;
+*self = *other;
+*other = *tmp;
+```
+
+according to \<^url>\<open>https://doc.rust-lang.org/src/core/cell.rs.html#364-375\<close> and
+\<^url>\<open>https://doc.rust-lang.org/src/core/ptr/mod.rs.html#373-388\<close>.
+\<close>
+
+(* We are omitting early return as we don't support it yet :( *)
+definition cell_swap_body :: "(cell_swap_env, 'p, rust_error) com" where
+  "cell_swap_body ==
+    \<comment> \<open>Initializing tmp with uninit\<close>
+    Basic (\<lambda>s. (let (r, s') = heap_new uninit s in s'\<lparr> tmp := r \<rparr>));;
+
+    \<comment> \<open>*tmp = *self\<close>
+    copy_betw_places self tmp;;
+    \<comment> \<open>*self = *other\<close>
+    copy_betw_places other self;;
+    \<comment> \<open>*self = *tmp\<close>
+    copy_betw_places tmp self
+"
+
+\<comment> \<open>A proof that shows self and val have the same value after Cell::set.\<close>
+lemma cell_set_value: "\<Gamma> \<turnstile>\<^sub>t
+  {s. wf_heap s
+  \<and> permission_is SharedReadWrite (self s) s
+  \<and> readable (val s) s}
+  cell_set_body
+  {s. memread (self s) s = memread (val s) s}"
+  unfolding cell_set_body_def
+  apply vcg
+  apply (auto simp add: Let_def)
+  by (metis nth_list_update_eq nth_list_update_neq)
+
+\<comment> \<open>A proof that shows self and return have the same value after Cell::get.\<close>
+lemma cell_get_value: "\<Gamma> \<turnstile>\<^sub>t
+  {s. wf_heap s
+  \<and> permission_is SharedReadWrite (self s) s
+  \<and> writable (return s) s}
+  cell_get_body
+  {s. memread (self s) s = memread (return s) s}"
+  unfolding cell_get_body_def
+  apply vcg
+  apply (auto simp add: Let_def)
+  using permission_is_imp_readable apply simp
+  by (metis nth_list_update_eq nth_list_update_neq)
+
+lemma cell_swap_value: "\<forall>x y. \<Gamma> \<turnstile>\<^sub>t
+  {s. wf_heap s
+  \<and> permission_is SharedReadWrite (self s) s
+  \<and> permission_is SharedReadWrite (other s) s
+  \<and> memread (self s) s = x
+  \<and> memread (other s) s = y}
+  cell_swap_body
+  {s. memread (self s) s = y \<and> memread (other s) s = x}"
+  unfolding cell_swap_body_def
+  apply vcg
+  oops
+
+end
